src/coq_formalism/graph_partial_order.v
@@ -18,16 +18,16 @@ Require Import Order.utilities.
 Section PO_Facts. 
 
 Context {measurement : Type}.
-Context {corruption : Type}.
+Context {adversary : Type}.
 
  (* Labels and States must have decidable equality *)
  Hypothesis eqDec_measurement : forall (x y : measurement), {x = y} + {x <> y}.
- Hypothesis eqDec_corruption : forall (x y : corruption), {x = y} + {x <> y}.
- Hypothesis eqDec_state : forall (G : attackgraph measurement corruption) (x y : G.(state _ _)), {x = y} + {x <> y}.
+ Hypothesis eqDec_adversary : forall (x y : adversary), {x = y} + {x <> y}.
+ Hypothesis eqDec_state : forall (G : attackgraph measurement adversary) (x y : G.(state _ _)), {x = y} + {x <> y}.
 
  (******* DEFINING PARTIAL ORDER (PO) ********
   **         =  \/  <   ->     <= *)
-Definition partial_order (G1 : attackgraph measurement corruption) (G2 : attackgraph measurement corruption) := 
+Definition partial_order (G1 : attackgraph measurement adversary) (G2 : attackgraph measurement adversary) := 
   bidir_homo G1 G2 \/ strict_partial_order G1 G2.
   
  (******* PROVE PO REFLEXIVE *********)
@@ -50,13 +50,13 @@ Qed.
  ** The following is a series of
  ** helper lemmas which prove 
  ** useful for transitivity *)
-Lemma cor_meas_label_ : forall  (G3 : attackgraph measurement corruption) (G2 : attackgraph measurement corruption) 
-(l : (list (state measurement corruption G3 * state measurement corruption G3))) m (l' : list (state measurement corruption G2 * state measurement corruption G2)) a,  label measurement corruption G3 (fst a) = inl m -> cor_subset_ind l' (a :: l) -> cor_subset_ind l' l.
+Lemma cor_meas_label_ : forall  (G3 : attackgraph measurement adversary) (G2 : attackgraph measurement adversary) 
+(l : (list (state measurement adversary G3 * state measurement adversary G3))) m (l' : list (state measurement adversary G2 * state measurement adversary G2)) a,  label measurement adversary G3 (fst a) = inl m -> cor_subset_ind l' (a :: l) -> cor_subset_ind l' l.
 Proof.
   intros. remember (a::l) as list1.   induction H0.
   + econstructor.   
   + econstructor.
-  ++ destruct (label measurement corruption G2 (fst x)) eqn:lab_x.
+  ++ destruct (label measurement adversary G2 (fst x)) eqn:lab_x.
   +++ destruct x. unfold find_cor. rewrite lab_x. apply I.
   +++ unfold find_cor. rewrite lab_x.
       unfold find_cor in *.
@@ -67,16 +67,16 @@ Proof.
   ++ intuition.
 Qed. 
 
-Lemma time_meas_label_ : forall  (G3 : attackgraph measurement corruption) (G2 : attackgraph measurement corruption) 
-(l : (list (state measurement corruption G3 * state measurement corruption G3))) m1 m2 c (l' : list (state measurement corruption G2 * state measurement corruption G2)) a,  ((label measurement corruption G3 (fst a) = inl m1 /\ label measurement corruption G3 (snd a) = inl m2) \/  (label measurement corruption G3 (fst a)) = inr c) -> time_subset_ind l' (a :: l) -> time_subset_ind l' l.
+Lemma time_meas_label_ : forall  (G3 : attackgraph measurement adversary) (G2 : attackgraph measurement adversary) 
+(l : (list (state measurement adversary G3 * state measurement adversary G3))) m1 m2 c (l' : list (state measurement adversary G2 * state measurement adversary G2)) a,  ((label measurement adversary G3 (fst a) = inl m1 /\ label measurement adversary G3 (snd a) = inl m2) \/  (label measurement adversary G3 (fst a)) = inr c) -> time_subset_ind l' (a :: l) -> time_subset_ind l' l.
 Proof.
   intros. remember (a::l) as list1. destruct H as [ms | cs].
   + induction H0.
   ++ econstructor.   
   ++ econstructor.
-  +++ unfold find_time. destruct (label measurement corruption G2 (fst x)) eqn:lab_x1;   
+  +++ unfold find_time. destruct (label measurement adversary G2 (fst x)) eqn:lab_x1;   
      eauto.
-     destruct (label measurement corruption G2 (snd (x))) eqn:lab_x2; eauto.
+     destruct (label measurement adversary G2 (snd (x))) eqn:lab_x2; eauto.
      unfold find_time in H. destruct ms as [m1' m2'].
      rewrite lab_x1 in H. rewrite lab_x2 in H. inversion H; subst.
   ++++ inversion H2; subst. destruct a. simpl in *. destruct H1. rewrite H1 in m2'. inversion m2'.
@@ -85,21 +85,21 @@ Proof.
   + induction H0.
   ++ econstructor.
   ++ econstructor; intuition.
-     unfold find_time. destruct (label measurement corruption G2 (fst x)) eqn:lab_x1; eauto. unfold find_time in H. rewrite lab_x1 in H.
-     destruct (label measurement corruption G2 (snd (x))) eqn:lab_x2; eauto.
+     unfold find_time. destruct (label measurement adversary G2 (fst x)) eqn:lab_x1; eauto. unfold find_time in H. rewrite lab_x1 in H.
+     destruct (label measurement adversary G2 (snd (x))) eqn:lab_x2; eauto.
      inversion H; subst.
   +++ inversion H3; subst. destruct a.  inversion H2; subst. simpl in *. rewrite H5 in cs. inversion cs.
   +++ inversion H3; subst. eauto.
 Qed. 
 
-Lemma cor_subset_not_nil_if_c : forall  (G3 : attackgraph measurement corruption) (G2 : attackgraph measurement corruption)  a (l : (list (state measurement corruption G3 * state measurement corruption G3))) (l' : (list (state measurement corruption G2 * state measurement corruption G2))) c, 
-l' = nil -> label measurement corruption G3 (fst a) = inr c -> cor_subset_ind (a :: l) l' -> False.
+Lemma cor_subset_not_nil_if_c : forall  (G3 : attackgraph measurement adversary) (G2 : attackgraph measurement adversary)  a (l : (list (state measurement adversary G3 * state measurement adversary G3))) (l' : (list (state measurement adversary G2 * state measurement adversary G2))) c, 
+l' = nil -> label measurement adversary G3 (fst a) = inr c -> cor_subset_ind (a :: l) l' -> False.
 Proof.
   intros. subst. simpl in *. inversion H1; subst.
   unfold find_cor in H3. rewrite H0 in H3. inversion H3.
 Qed. 
 
-Lemma po_trans_helper : forall (G1 G2 G3 : attackgraph measurement corruption), bidir_homo G1 G2 /\ strict_partial_order G2 G3 -> strict_partial_order G1 G3.
+Lemma po_trans_helper : forall (G1 G2 G3 : attackgraph measurement adversary), bidir_homo G1 G2 /\ strict_partial_order G2 G3 -> strict_partial_order G1 G3.
 Proof with intuition.
 intros... 
 unfold bidir_homo in H0.
@@ -109,36 +109,36 @@ destruct spoG1G2. unfold homomorphism in H. destruct H as [gste glab].
 unfold strict_partial_order in *...
 (* goal: cor subset *)
 + clear H. clear H2. clear gste.
-  induction (steps measurement corruption G1); econstructor.
+  induction (steps measurement adversary G1); econstructor.
 ++ destruct a.
   eapply find_cor_helper;  eauto.
   unfold find_cor.
-  destruct (label measurement corruption G1 (fst (s, s0))) eqn:lab'; eauto.
+  destruct (label measurement adversary G1 (fst (s, s0))) eqn:lab'; eauto.
   simpl in *. intuition. clear IHl.
   clear H1.
   specialize ste with s s0.
   intuition. 
-  induction (steps measurement corruption G2)...
+  induction (steps measurement adversary G2)...
   simpl in *. inversion H1.
-  simpl in *. destruct a... 
+  simpl in *. destruct a0... 
 +++ inversion H. econstructor. specialize lab with s s0...
     rewrite <- lab'. rewrite H1. eauto.
 +++ apply ex_tail. eapply IHl0; intuition; specialize glab with st1 st2...
 ++ apply IHl; auto with *.
   (* goal: time subset  *)
 +  clear H. clear H1. clear gste.
-      induction (steps measurement corruption G1); econstructor.
+      induction (steps measurement adversary G1); econstructor.
 ++ destruct a.
       eapply find_time_helper; eauto.
       unfold find_time.
-      destruct (label measurement corruption G1 (fst (s, s0))) eqn:fst; eauto.
-      destruct (label measurement corruption G1 (snd (s, s0))) eqn:snd; eauto.
+      destruct (label measurement adversary G1 (fst (s, s0))) eqn:fst; eauto.
+      destruct (label measurement adversary G1 (snd (s, s0))) eqn:snd; eauto.
       simpl in *... clear IHl. clear H2.
       specialize ste with s s0.
       intuition. 
-      induction (steps measurement corruption G2).
+      induction (steps measurement adversary G2).
       simpl in *. inversion H1.
-      simpl in *. destruct a...
+      simpl in *. destruct a0...
 +++ inversion H. econstructor. split; specialize lab with s s0;
       intuition. rewrite <- snd. rewrite H6. eauto.
        rewrite <- fst. rewrite H1. eauto.
@@ -149,33 +149,33 @@ unfold strict_partial_order in *...
 + left.
   unfold cor_proper_subset. intuition.
 ++ unfold cor_proper_subset in H... clear H2. clear H1. clear H3. clear gste.
-  induction (steps measurement corruption G1); econstructor.
+  induction (steps measurement adversary G1); econstructor.
 +++ destruct a.
       eapply find_cor_helper;  eauto.
       unfold find_cor.
-      destruct (label measurement corruption G1 (fst (s, s0))) eqn:lab'; eauto.
+      destruct (label measurement adversary G1 (fst (s, s0))) eqn:lab'; eauto.
       simpl in *. intuition. clear IHl. clear H0.
       specialize ste with s s0.
       intuition. 
-      induction (steps measurement corruption G2).
+      induction (steps measurement adversary G2).
       simpl in *. inversion H1.
-      simpl in *. destruct a...
+      simpl in *. destruct a0...
 ++++ inversion H. econstructor. specialize lab with s s0.
       intuition. rewrite <- lab'. rewrite H1. eauto.
 ++++ apply ex_tail. eapply IHl0; intuition; specialize glab with st1 st2...
 +++ apply IHl; auto with *.
 ++ unfold cor_proper_subset in H... apply H4.
   clear H4. clear H1. clear H2. clear H3. clear gste. 
-  induction (steps measurement corruption G3); econstructor. 
+  induction (steps measurement adversary G3); econstructor. 
 +++ destruct a.
   inversion H0; subst.
   eapply find_cor_helper; eauto. clear IHl. clear H4. clear H2. clear H0.
-  induction (steps measurement corruption G1); econstructor.
+  induction (steps measurement adversary G1); econstructor.
 ++++ unfold find_cor in *. 
-    destruct (label measurement corruption G1 (fst a)) eqn:lab'; eauto.
+    destruct (label measurement adversary G1 (fst a)) eqn:lab'; eauto.
     destruct a. specialize lab with s1 s2... simpl in *...
     specialize ste with s1 s2. simpl in *... clear IHl0.  (* clear IHl0. clear H4. clear H.*)
-    induction (steps measurement corruption G2).
+    induction (steps measurement adversary G2).
     inversion H4.
     simpl in *.
     destruct H4.
@@ -185,36 +185,36 @@ unfold strict_partial_order in *...
     specialize glab with st1 st2. simpl in *...
 ++++ apply IHl0; auto with *.  
 +++ eapply IHl. inversion H0...
-(* goal corruption subset *)
+(* goal adversary subset *)
 + clear H. clear H2. clear gste.
-induction (steps measurement corruption G1); econstructor.
+induction (steps measurement adversary G1); econstructor.
 ++ destruct a.
   eapply find_cor_helper;  eauto.
   unfold find_cor.
-  destruct (label measurement corruption G1 (fst (s, s0))) eqn:lab'; eauto.
+  destruct (label measurement adversary G1 (fst (s, s0))) eqn:lab'; eauto.
   simpl in *. intuition. clear IHl.
   clear H1. specialize ste with s s0. intuition. 
-  induction (steps measurement corruption G2)...
+  induction (steps measurement adversary G2)...
   simpl in *. inversion H1.
-  simpl in *. destruct a... 
+  simpl in *. destruct a0... 
 +++ inversion H. econstructor. specialize lab with s s0...
   rewrite <- lab'. rewrite H1. eauto.
 +++ apply ex_tail. eapply IHl0; intuition; specialize glab with st1 st2...
 ++ apply IHl; auto with *.
 + (* goal : time subset *) 
   clear H. clear H1. clear gste.
-      induction (steps measurement corruption G1); econstructor.
+      induction (steps measurement adversary G1); econstructor.
 ++ destruct a.
       eapply find_time_helper; eauto.
       unfold find_time.
-      destruct (label measurement corruption G1 (fst (s, s0))) eqn:fst; eauto.
-      destruct (label measurement corruption G1 (snd (s, s0))) eqn:snd; eauto.
+      destruct (label measurement adversary G1 (fst (s, s0))) eqn:fst; eauto.
+      destruct (label measurement adversary G1 (snd (s, s0))) eqn:snd; eauto.
       simpl in *... clear IHl. clear H2.
       specialize ste with s s0.
       intuition. 
-      induction (steps measurement corruption G2).
+      induction (steps measurement adversary G2).
       simpl in *. inversion H1.
-      simpl in *. destruct a...
+      simpl in *. destruct a0...
 +++ inversion H. econstructor. split; specialize lab with s s0;
       intuition. rewrite <- snd. rewrite H6. eauto.
        rewrite <- fst. rewrite H1. eauto.
@@ -225,16 +225,16 @@ induction (steps measurement corruption G1); econstructor.
 + right.
   unfold time_proper_subset. intuition.
 ++ unfold time_proper_subset in H... clear H2. clear H1. clear H3. clear gste.
-  induction (steps measurement corruption G1); econstructor.
+  induction (steps measurement adversary G1); econstructor.
 +++ destruct a.
   eapply find_time_helper;  eauto; unfold find_time.
-  destruct (label measurement corruption G1 (fst (s, s0))) eqn:lab'; eauto.
-  destruct (label measurement corruption G1 (snd (s, s0))) eqn:lab''; eauto.
+  destruct (label measurement adversary G1 (fst (s, s0))) eqn:lab'; eauto.
+  destruct (label measurement adversary G1 (snd (s, s0))) eqn:lab''; eauto.
   simpl in *... clear IHl. clear H0.
   specialize ste with s s0...
-  induction (steps measurement corruption G2).
+  induction (steps measurement adversary G2).
   simpl in *. inversion H1.
-  simpl in *. destruct a...
+  simpl in *. destruct a0...
 ++++ inversion H. econstructor. specialize lab with s s0.
 intuition. rewrite <- lab''. rewrite H6. eauto.
 rewrite <- lab'. rewrite H1...
@@ -242,17 +242,17 @@ rewrite <- lab'. rewrite H1...
 +++ apply IHl; auto with *.
 ++ unfold time_proper_subset in H... apply H4.
 clear H4. clear H1. clear H2. clear H3. clear gste. 
-induction (steps measurement corruption G3); econstructor. 
+induction (steps measurement adversary G3); econstructor. 
 +++ destruct a.
 inversion H0; subst.
 eapply find_time_helper; eauto. clear IHl. clear H4. clear H2. clear H0.
-induction (steps measurement corruption G1); econstructor.
+induction (steps measurement adversary G1); econstructor.
 ++++ unfold find_time in *. 
-destruct (label measurement corruption G1 (fst a)) eqn:lab'; eauto.
-destruct (label measurement corruption G1 (snd a)) eqn:lab''; eauto.
+destruct (label measurement adversary G1 (fst a)) eqn:lab'; eauto.
+destruct (label measurement adversary G1 (snd a)) eqn:lab''; eauto.
 destruct a. specialize lab with s1 s2... simpl in *...
 specialize ste with s1 s2. simpl in *... clear IHl0.  (* clear IHl0. clear H4. clear H.*)
-induction (steps measurement corruption G2).
+induction (steps measurement adversary G2).
 inversion H4. simpl in *. destruct H4.
 +++++ destruct a. inversion H1. apply ex_head... rewrite <- lab''. rewrite H2. reflexivity.
       rewrite <- lab'. rewrite H...
@@ -263,7 +263,7 @@ specialize glab with st1 st2. simpl in *...
 +++ eapply IHl. inversion H0...
 Qed.
 
-Lemma po_trans_helper' : forall (G1 G2 G3 : attackgraph measurement corruption), strict_partial_order G1 G2 /\ bidir_homo G2 G3 -> strict_partial_order G1 G3.
+Lemma po_trans_helper' : forall (G1 G2 G3 : attackgraph measurement adversary), strict_partial_order G1 G2 /\ bidir_homo G2 G3 -> strict_partial_order G1 G3.
 Proof with intuition.
 intros G1 G2 G3 H1. destruct H1 as [H1 H0]. 
 unfold bidir_homo in H0.
@@ -273,34 +273,34 @@ destruct spoG1G2. unfold homomorphism in H. destruct H as [gste glab].
 unfold strict_partial_order in *...
 (* goal: cor subset *)
 + clear H. clear H2. clear gste.
-  induction (steps measurement corruption G1); econstructor.
+  induction (steps measurement adversary G1); econstructor.
 ++ destruct a.
    inversion H1; subst.  
    eapply find_cor_helper;  eauto.
     unfold find_cor. clear IHl. clear H1. clear H2. clear H4. clear glab. 
-    induction (steps measurement corruption G2); econstructor.
-+++ destruct a.  unfold find_cor. destruct (label measurement corruption G2 (fst (s1, s2))) eqn:lab'; eauto. simpl in *.
+    induction (steps measurement adversary G2); econstructor.
++++ destruct a.  unfold find_cor. destruct (label measurement adversary G2 (fst (s1, s2))) eqn:lab'; eauto. simpl in *.
     specialize lab with s1 s2.
     specialize ste with s1 s2. simpl in *... clear IHl0.
-    induction (steps measurement corruption G3)... inversion H1. simpl in *...
-    econstructor. destruct a. inversion H3. rewrite <- lab'. rewrite H... apply ex_tail...
+    induction (steps measurement adversary G3)... inversion H1. simpl in *...
+    econstructor. destruct a0. inversion H3. rewrite <- lab'. rewrite H... apply ex_tail...
 +++ apply IHl0; auto with *.
 ++ inversion H1...
 + (* goal: time subset *) 
   clear H. clear H1. clear gste.
-  induction (steps measurement corruption G1); econstructor.
+  induction (steps measurement adversary G1); econstructor.
 ++ destruct a.
    inversion H2; subst.  
    eapply find_time_helper;  eauto. clear IHl. clear H1. clear H2. clear H4. clear glab. 
-    induction (steps measurement corruption G2); econstructor.
+    induction (steps measurement adversary G2); econstructor.
 +++ destruct a.  unfold find_time. 
-   destruct (label measurement corruption G2 (fst (s1, s2))) eqn:lab'; eauto. 
-   destruct (label measurement corruption G2 (snd (s1, s2))) eqn:lab''; eauto. simpl in *.
+   destruct (label measurement adversary G2 (fst (s1, s2))) eqn:lab'; eauto. 
+   destruct (label measurement adversary G2 (snd (s1, s2))) eqn:lab''; eauto. simpl in *.
     specialize lab with s1 s2.
     specialize ste with s1 s2. simpl in *... clear IHl0.
-    induction (steps measurement corruption G3)... inversion H1.
+    induction (steps measurement adversary G3)... inversion H1.
     simpl in *...
-    econstructor. destruct a. inversion H3...
+    econstructor. destruct a0. inversion H3...
      rewrite <- lab''; rewrite H4...
      rewrite <- lab'; rewrite H...
     apply ex_tail...
@@ -309,32 +309,32 @@ unfold strict_partial_order in *...
 (* goal: cor proper *)
 + left. unfold cor_proper_subset in *...
 ++ clear H3. clear H2. clear H1. clear gste.
-  induction (steps measurement corruption G1); econstructor.
+  induction (steps measurement adversary G1); econstructor.
 +++ destruct a.
    inversion H0; subst.  
    eapply find_cor_helper;  eauto.
    clear IHl. clear H0. clear H2. clear H4. clear glab. 
-    induction (steps measurement corruption G2); econstructor.
-++++ destruct a.  unfold find_cor. destruct (label measurement corruption G2 (fst (s1, s2))) eqn:lab'; eauto. simpl in *.
+    induction (steps measurement adversary G2); econstructor.
+++++ destruct a.  unfold find_cor. destruct (label measurement adversary G2 (fst (s1, s2))) eqn:lab'; eauto. simpl in *.
     specialize lab with s1 s2.
     specialize ste with s1 s2. simpl in *... clear IHl0.
-    induction (steps measurement corruption G3)... inversion H1.
+    induction (steps measurement adversary G3)... inversion H1.
     simpl in *...
-    econstructor. destruct a. inversion H3. rewrite <- lab'.
+    econstructor. destruct a0. inversion H3. rewrite <- lab'.
     rewrite H...
     apply ex_tail...
 ++++ apply IHl0; auto with *.
 +++ inversion H0...
 ++ apply H3. clear H1. clear H2. clear H0. clear H3.
    clear gste.
-   induction (steps measurement corruption G2); econstructor.
+   induction (steps measurement adversary G2); econstructor.
 +++ eapply find_cor_helper; eauto. destruct a.
-    unfold find_cor. destruct (label measurement corruption G2 (fst (s,s0))) eqn:lab'; eauto.
+    unfold find_cor. destruct (label measurement adversary G2 (fst (s,s0))) eqn:lab'; eauto.
     specialize lab with s s0... simpl in *...
     specialize ste with s s0. simpl in *... clear IHl.  (* clear IHl0. clear H4. clear H.*)
-    induction (steps measurement corruption G3).
+    induction (steps measurement adversary G3).
     inversion H5. simpl in *. destruct H5.
-    destruct a. inversion H2. apply ex_head. rewrite <- lab'. rewrite H0...
+    destruct a0. inversion H2. apply ex_head. rewrite <- lab'. rewrite H0...
     apply ex_tail. eapply IHl0... auto with *.
     specialize glab with st1 st2. simpl in *...  
     specialize glab with st1 st2. simpl in *...
@@ -342,34 +342,34 @@ unfold strict_partial_order in *...
 +++ apply IHl; auto with *.  
 (* goal: cor subset *)
 + clear H. clear H2. clear gste.
-  induction (steps measurement corruption G1); econstructor.
+  induction (steps measurement adversary G1); econstructor.
 ++ destruct a.
    inversion H1; subst.  
    eapply find_cor_helper;  eauto.
     unfold find_cor. clear IHl. clear H1. clear H2. clear H4. clear glab. 
-    induction (steps measurement corruption G2); econstructor.
-+++ destruct a.  unfold find_cor. destruct (label measurement corruption G2 (fst (s1, s2))) eqn:lab'; eauto. simpl in *.
+    induction (steps measurement adversary G2); econstructor.
++++ destruct a.  unfold find_cor. destruct (label measurement adversary G2 (fst (s1, s2))) eqn:lab'; eauto. simpl in *.
     specialize lab with s1 s2.
     specialize ste with s1 s2. simpl in *... clear IHl0.
-    induction (steps measurement corruption G3)... inversion H1. simpl in *...
-    econstructor. destruct a. inversion H3. rewrite <- lab'. rewrite H... apply ex_tail...
+    induction (steps measurement adversary G3)... inversion H1. simpl in *...
+    econstructor. destruct a0. inversion H3. rewrite <- lab'. rewrite H... apply ex_tail...
 +++ apply IHl0; auto with *.
 ++ inversion H1...
 + (* goal: time subset *) 
   clear H. clear H1. clear gste.
-  induction (steps measurement corruption G1); econstructor.
+  induction (steps measurement adversary G1); econstructor.
 ++ destruct a.
    inversion H2; subst.  
    eapply find_time_helper;  eauto. clear IHl. clear H1. clear H2. clear H4. clear glab. 
-    induction (steps measurement corruption G2); econstructor.
+    induction (steps measurement adversary G2); econstructor.
 +++ destruct a.  unfold find_time. 
-   destruct (label measurement corruption G2 (fst (s1, s2))) eqn:lab'; eauto. 
-   destruct (label measurement corruption G2 (snd (s1, s2))) eqn:lab''; eauto. simpl in *.
+   destruct (label measurement adversary G2 (fst (s1, s2))) eqn:lab'; eauto. 
+   destruct (label measurement adversary G2 (snd (s1, s2))) eqn:lab''; eauto. simpl in *.
     specialize lab with s1 s2.
     specialize ste with s1 s2. simpl in *... clear IHl0.
-    induction (steps measurement corruption G3)... inversion H1.
+    induction (steps measurement adversary G3)... inversion H1.
     simpl in *...
-    econstructor. destruct a. inversion H3...
+    econstructor. destruct a0. inversion H3...
      rewrite <- lab''; rewrite H4...
      rewrite <- lab'; rewrite H...
     apply ex_tail...
@@ -378,37 +378,37 @@ unfold strict_partial_order in *...
 (* goal: time proper *)
 + right. unfold time_proper_subset in *...
 ++ clear H1. clear H2. clear H3. clear gste.
-  induction (steps measurement corruption G1); econstructor.
+  induction (steps measurement adversary G1); econstructor.
 +++ destruct a.
    inversion H0; subst.  
    eapply find_time_helper;  eauto.
    clear IHl. clear H0. clear H2. clear H4. clear glab. 
-    induction (steps measurement corruption G2); econstructor.
+    induction (steps measurement adversary G2); econstructor.
 ++++ destruct a.  unfold find_time. 
-     destruct (label measurement corruption G2 (fst (s1, s2))) eqn:lab'; eauto.
-     destruct (label measurement corruption G2 (snd (s1, s2))) eqn:lab''; eauto.
+     destruct (label measurement adversary G2 (fst (s1, s2))) eqn:lab'; eauto.
+     destruct (label measurement adversary G2 (snd (s1, s2))) eqn:lab''; eauto.
      simpl in *.
     specialize lab with s1 s2.
     specialize ste with s1 s2. simpl in *... clear IHl0.
-    induction (steps measurement corruption G3)... inversion H1.
+    induction (steps measurement adversary G3)... inversion H1.
     simpl in *...
-    econstructor. destruct a; inversion H3... rewrite <- lab''. rewrite H4...
+    econstructor. destruct a0; inversion H3... rewrite <- lab''. rewrite H4...
     rewrite <- lab'. rewrite H... 
     apply ex_tail...
 ++++ apply IHl0; auto with *.
 +++ inversion H0...
 ++ apply H3. clear H1. clear H2. clear H0. clear H3.
    clear gste.
-   induction (steps measurement corruption G2); econstructor.
+   induction (steps measurement adversary G2); econstructor.
 +++ eapply find_time_helper; eauto. destruct a.
     unfold find_time. 
-    destruct (label measurement corruption G2 (fst (s,s0))) eqn:lab'; eauto.
-    destruct (label measurement corruption G2 (snd (s, s0))) eqn:lab''; eauto.
+    destruct (label measurement adversary G2 (fst (s,s0))) eqn:lab'; eauto.
+    destruct (label measurement adversary G2 (snd (s, s0))) eqn:lab''; eauto.
     specialize lab with s s0... simpl in *...
     specialize ste with s s0. simpl in *... clear IHl.  (* clear IHl0. clear H4. clear H.*)
-    induction (steps measurement corruption G3).
+    induction (steps measurement adversary G3).
     inversion H5. simpl in *. destruct H5.
-    destruct a. inversion H2. apply ex_head. rewrite <- lab'. rewrite H0...
+    destruct a0. inversion H2. apply ex_head. rewrite <- lab'. rewrite H0...
     rewrite <- lab''. rewrite H3...
     apply ex_tail. eapply IHl0... auto with *.
     specialize glab with st1 st2. simpl in *...  
