src/coq_formalism/useless_code/main.v
@@ -13,23 +13,23 @@ Date: Sept 11, 2023 *)
 
 Require Import Coq.Lists.List.
 
-(* Attack graph is parameterized over measurement and corruption events *)
-Record attackgraph (measurement corruption : Type) : Type := 
+(* Attack graph is parameterized over measurement and adversary events *)
+Record attackgraph (measurement adversary : Type) : Type := 
 {
     state : Type ;
     steps : list (state * state) ;
-    label : state -> measurement + corruption
+    label : state -> measurement + adversary
 }.
 
 Section Reducer.
 
     Context {measurement : Type}.
-    Context {corruption : Type}.
-    Context {G : attackgraph measurement corruption}.
+    Context {adversary : Type}.
+    Context {G : attackgraph measurement adversary}.
 
     (* Labels and States must have decidable equality *)
     Hypothesis eqDec_measurement : forall (x y : measurement), {x = y} + {x <> y}.
-    Hypothesis eqDec_corruption : forall (x y : corruption), {x = y} + {x <> y}.
+    Hypothesis eqDec_adversary : forall (x y : adversary), {x = y} + {x <> y}.
     Hypothesis eqDec_state : forall (x y : G.(state _ _)), {x = y} + {x <> y}.
 
     (* steps are equivalent or not equivalent *)
@@ -137,15 +137,15 @@ End Reducer.
 Section Comparison. 
 
 Context {measurement : Type}.
-Context {corruption : Type}.
+Context {adversary : Type}.
 (* need two attack graphs for comparison now 
-Context {G : attackgraph measurement corruption}.
-Context {G2 : attackgraph measurement corruption}. *)
+Context {G : attackgraph measurement adversary}.
+Context {G2 : attackgraph measurement adversary}. *)
 
 (* Labels and States must have decidable equality *)
 Hypothesis eqDec_measurement : forall (x y : measurement), {x = y} + {x <> y}.
-Hypothesis eqDec_corruption : forall (x y : corruption), {x = y} + {x <> y}.
-Hypothesis eqDec_state : forall (G : attackgraph measurement corruption) (x y : G.(state _ _)), {x = y} + {x <> y}.
+Hypothesis eqDec_adversary : forall (x y : adversary), {x = y} + {x <> y}.
+Hypothesis eqDec_state : forall (G : attackgraph measurement adversary) (x y : G.(state _ _)), {x = y} + {x <> y}.
 
 Print eqDec_step.
 
@@ -217,14 +217,14 @@ Qed.
     DEFINING SUBSETS 
 
 We say a is strictly less than b (a < b) if 
-* 1. b has more corruption events 
+* 1. b has more adversary events 
 * OR 
-* 2. b has more time constrained corruption events *)
+* 2. b has more time constrained adversary events *)
 
-(****** MORE CORRUPTION EVENTS SUBSET *)
+(****** MORE adversary EVENTS SUBSET *)
 
-(* corruption events of x are a subset of corruption events in y *)
-Fixpoint cor_subset {G1 G2 : attackgraph measurement corruption} 
+(* adversary events of x are a subset of adversary events in y *)
+Fixpoint cor_subset {G1 G2 : attackgraph measurement adversary} 
                 (x : list (G1.(state _ _) * G1.(state _ _))) (y : list (G2.(state _ _) * G2.(state _ _))) : Prop :=
   match x with 
   | nil => True
@@ -238,12 +238,12 @@ Fixpoint cor_subset {G1 G2 : attackgraph measurement corruption}
 (* existsb _ (fun st2 => G2.(label _ _) st2 = inr c) (fst (split y)) *)
 
 (* Proper subset using the fixpoint definition *)
-Definition cor_proper_subset' {G1 G2 : attackgraph measurement corruption} 
+Definition cor_proper_subset' {G1 G2 : attackgraph measurement adversary} 
 (x : list (G1.(state _ _) * G1.(state _ _))) (y : list (G2.(state _ _) * G2.(state _ _))) := cor_subset x y /\ ~ cor_subset y x. 
 
-(* determine if corruption event in G1 is present in y
+(* determine if adversary event in G1 is present in y
  * input: one state in G1 (no need to recurse through G1) and list to search (y) *)
-Definition find_cor {G1 G2 : attackgraph measurement corruption} (st : G1.(state _ _)) (y : list (G2.(state _ _) * G2.(state _ _))) : Prop := 
+Definition find_cor {G1 G2 : attackgraph measurement adversary} (st : G1.(state _ _)) (y : list (G2.(state _ _) * G2.(state _ _))) : Prop := 
     match (G1.(label _ _) st) with 
     | inr c => existsb_ind _ (fun step => match step with 
                                     | (st2, _ ) => G2.(label _ _) st2 = inr c
@@ -251,8 +251,8 @@ Definition find_cor {G1 G2 : attackgraph measurement corruption} (st : G1.(state
     | inl r => True 
     end. 
 
-(* Inductively defined corruption subset *)
-Inductive cor_subset_ind {G1 G2 : attackgraph measurement corruption} : 
+(* Inductively defined adversary subset *)
+Inductive cor_subset_ind {G1 G2 : attackgraph measurement adversary} : 
 list (G1.(state _ _) * G1.(state _ _)) -> (list (G2.(state _ _) * G2.(state _ _))) -> Prop :=
 | sub_nil : forall y, cor_subset_ind nil y
 | sub_head : forall x xs y, find_cor (fst x) y -> cor_subset_ind xs y -> cor_subset_ind (x::xs) y.
@@ -263,7 +263,7 @@ Proof.
 (* proof won't work bc (a::x) could be list of measurement events *)
 Abort.
 
-(* If corruption event is in xs then it is in (x::xs) *)
+(* If adversary event is in xs then it is in (x::xs) *)
 Lemma find_cons : forall G1 (x0: (G1.(state _ _) * G1.(state _ _))) x (xs : list (G1.(state _ _) * G1.(state _ _))), 
     find_cor (fst x0) (xs) -> find_cor (fst x0) (x :: xs).
 Proof.
@@ -275,7 +275,7 @@ Qed.
 
 (* Need this helper lemma to prove transitivity *)
 Lemma find_cor_helper : forall G1 G2 G3 (x: (G1.(state _ _) * G1.(state _ _)))
-                         (ys:list (state measurement corruption G2 * state measurement corruption G2)), 
+                         (ys:list (state measurement adversary G2 * state measurement adversary G2)), 
                          find_cor (fst x) (ys) -> forall (zs : list (G3.(state _ _) * G3.(state _ _))), cor_subset_ind ys zs -> find_cor (fst x) zs.
 Proof.
     intros G1 G2 G3 x ys H. intros. 
@@ -331,32 +331,32 @@ Proof.
 Qed.
 
 (* Proper subset using the inductive definition *)
-Definition cor_proper_subset {G1 G2 : attackgraph measurement corruption} 
+Definition cor_proper_subset {G1 G2 : attackgraph measurement adversary} 
 (x : list (G1.(state _ _) * G1.(state _ _))) (y : list (G2.(state _ _) * G2.(state _ _))) := cor_subset_ind x y /\ ~ cor_subset_ind y x. 
 
 (*******************************************
-Prove the proper subset of corruption events is a strict partial order *)
+Prove the proper subset of adversary events is a strict partial order *)
 
-(* define strictly less for corruption events as a proper subset relation *) 
+(* define strictly less for adversary events as a proper subset relation *) 
 (* Class strict_partial_order {X : Type} (R : X -> X -> Prop) := {
     irreflexive := forall a : X, ~ R a a ; 
     asymmetric := forall a b : X, R a b -> ~ R b a ;
     transitive := forall a b c: X, R a b -> R b c -> R a c 
     }. *)
     
-Theorem cor_irr : forall (g1 : attackgraph measurement corruption) (x : list (g1.(state _ _) * g1.(state _ _)) ), ~ cor_proper_subset x x.
+Theorem cor_irr : forall (g1 : attackgraph measurement adversary) (x : list (g1.(state _ _) * g1.(state _ _)) ), ~ cor_proper_subset x x.
     Proof.
     intros. unfold cor_proper_subset. unfold not. intros. inversion H. contradiction.
     Qed.
 
-Theorem cor_asym : forall (g1 g2 : attackgraph measurement corruption)  (x : list (g1.(state _ _) * g1.(state _ _)) ) (y : list (g2.(state _ _) * g2.(state _ _)) ), cor_proper_subset x y -> ~ cor_proper_subset y x.
+Theorem cor_asym : forall (g1 g2 : attackgraph measurement adversary)  (x : list (g1.(state _ _) * g1.(state _ _)) ) (y : list (g2.(state _ _) * g2.(state _ _)) ), cor_proper_subset x y -> ~ cor_proper_subset y x.
     Proof.
     intros. unfold cor_proper_subset in *. inversion H. unfold not. intros. inversion H2. auto.
     Qed.
 
 Ltac invc H := inversion H; clear H.  
 
-Theorem cor_trans : forall (g1 g2 g3 : attackgraph measurement corruption) (xs : list (g1.(state _ _) * g1.(state _ _)) ) (ys : list (g2.(state _ _) * g2.(state _ _)) ), 
+Theorem cor_trans : forall (g1 g2 g3 : attackgraph measurement adversary) (xs : list (g1.(state _ _) * g1.(state _ _)) ) (ys : list (g2.(state _ _) * g2.(state _ _)) ), 
 cor_proper_subset xs ys -> 
 forall (zs : list (g3.(state _ _) * g3.(state _ _)) ), cor_proper_subset ys zs -> 
 cor_proper_subset xs zs.
@@ -366,10 +366,10 @@ cor_proper_subset xs zs.
     + unfold not. intros. intuition. apply H4. eapply cor_subset_ind_trans; eauto.
     Qed. 
 
-(****** TIME CONSTRAINED CORRUPTION EVENT SUBSET *)
+(****** TIME CONSTRAINED adversary EVENT SUBSET *)
 
-(* corruption events of x are a subset of corruption events in y *)
-Fixpoint time_subset {G1 G2 : attackgraph measurement corruption} 
+(* adversary events of x are a subset of adversary events in y *)
+Fixpoint time_subset {G1 G2 : attackgraph measurement adversary} 
                 (x : list (G1.(state _ _) * G1.(state _ _))) (y : list (G2.(state _ _) * G2.(state _ _))) : Prop :=
     match x with 
     | nil => True
@@ -381,9 +381,9 @@ Fixpoint time_subset {G1 G2 : attackgraph measurement corruption}
                         end
     end.
 
-(* determine if a time constrained corruption event in G1 is present in y
+(* determine if a time constrained adversary event in G1 is present in y
 * input: one step in G1 (no need to recurse through G1) and list to search (y) *)
-Definition find_time {G1 G2 : attackgraph measurement corruption} (st1 : G1.(state _ _) *  G1.(state _ _)) (y : list (G2.(state _ _) * G2.(state _ _))) : Prop := 
+Definition find_time {G1 G2 : attackgraph measurement adversary} (st1 : G1.(state _ _) *  G1.(state _ _)) (y : list (G2.(state _ _) * G2.(state _ _))) : Prop := 
     match G1.(label _ _) (fst(st1)) , G1.(label _ _) (snd(st1))  with 
     | inl m , inr c => ( existsb_ind _ (fun step => match step with 
                                     | (st1', st2') => G2.(label _ _) st2' = inr c /\ G2.(label _ _) st1' = inl m
@@ -391,8 +391,8 @@ Definition find_time {G1 G2 : attackgraph measurement corruption} (st1 : G1.(sta
     | _ , _ => True 
     end. 
 
-(* Inductively defined corruption subset *)
-Inductive time_subset_ind {G1 G2 : attackgraph measurement corruption} : 
+(* Inductively defined adversary subset *)
+Inductive time_subset_ind {G1 G2 : attackgraph measurement adversary} : 
 list (G1.(state _ _) * G1.(state _ _)) -> (list (G2.(state _ _) * G2.(state _ _))) -> Prop :=
 | time_nil : forall y, time_subset_ind nil y
 | time_head : forall x xs y, find_time x y -> time_subset_ind xs y -> time_subset_ind (x::xs) y.
@@ -434,7 +434,7 @@ Proof.
 Qed.
 
 Lemma find_time_helper : forall G1 G2 G3 (x: (G1.(state _ _) * G1.(state _ _)))
-                         (ys:list (state measurement corruption G2 * state measurement corruption G2)), 
+                         (ys:list (state measurement adversary G2 * state measurement adversary G2)), 
                          find_time x ys -> forall (zs : list (G3.(state _ _) * G3.(state _ _))), time_subset_ind ys zs -> find_time x zs.
 Proof.
     intros G1 G2 G3 x ys H. intros. 
@@ -453,7 +453,7 @@ Proof.
     ++++ destruct y. simpl in *.
          inversion H3. rewrite H in contra. inversion contra.
          rewrite H2 in Hfst. inversion Hfst. subst. auto.
-    (* fst y is a corruption event *)
+    (* fst y is a adversary event *)
     +++ destruct (G2.(label _ _) (snd y)) eqn:contra ; auto.
     ++++ destruct y. intuition. simpl in *. rewrite Hfst in H2. inversion H2.
     ++++ destruct y. intuition. simpl in *. rewrite Hfst in H2. inversion H2. 
@@ -474,20 +474,20 @@ Proof.
 Qed.
 
 (* Proper subset using the inductive definition *)
-Definition time_proper_subset {G1 G2 : attackgraph measurement corruption} 
+Definition time_proper_subset {G1 G2 : attackgraph measurement adversary} 
 (x : list (G1.(state _ _) * G1.(state _ _))) (y : list (G2.(state _ _) * G2.(state _ _))) := time_subset_ind x y /\ ~ time_subset_ind y x.
 
-Theorem time_irr : forall (g1 : attackgraph measurement corruption) (x : list (g1.(state _ _) * g1.(state _ _)) ), ~ time_proper_subset x x.
+Theorem time_irr : forall (g1 : attackgraph measurement adversary) (x : list (g1.(state _ _) * g1.(state _ _)) ), ~ time_proper_subset x x.
 Proof.
     intros. unfold time_proper_subset. unfold not. intros. inversion H. contradiction.
 Qed.
 
-Theorem time_asym : forall (g1 g2 : attackgraph measurement corruption)  (x : list (g1.(state _ _) * g1.(state _ _)) ) (y : list (g2.(state _ _) * g2.(state _ _)) ), time_proper_subset x y -> ~ time_proper_subset y x.
+Theorem time_asym : forall (g1 g2 : attackgraph measurement adversary)  (x : list (g1.(state _ _) * g1.(state _ _)) ) (y : list (g2.(state _ _) * g2.(state _ _)) ), time_proper_subset x y -> ~ time_proper_subset y x.
 Proof.
     intros. unfold time_proper_subset in *. inversion H. unfold not. intros. inversion H2. auto.
 Qed.
 
-Theorem time_trans : forall (g1 g2 g3 : attackgraph measurement corruption) (xs : list (g1.(state _ _) * g1.(state _ _)) ) (ys : list (g2.(state _ _) * g2.(state _ _)) ), 
+Theorem time_trans : forall (g1 g2 g3 : attackgraph measurement adversary) (xs : list (g1.(state _ _) * g1.(state _ _)) ) (ys : list (g2.(state _ _) * g2.(state _ _)) ), 
 time_proper_subset xs ys -> 
 forall (zs : list (g3.(state _ _) * g3.(state _ _)) ), time_proper_subset ys zs -> 
 time_proper_subset xs zs.
@@ -497,17 +497,17 @@ Proof.
     + unfold not. intros. intuition. apply H4. eapply time_subset_ind_trans; eauto.
 Qed. 
 
-Definition strict_partial_order {g1 g2 : attackgraph measurement corruption} (xs : list (g1.(state _ _) * g1.(state _ _)) ) (ys : list (g2.(state _ _) * g2.(state _ _))) : Prop := 
+Definition strict_partial_order {g1 g2 : attackgraph measurement adversary} (xs : list (g1.(state _ _) * g1.(state _ _)) ) (ys : list (g2.(state _ _) * g2.(state _ _))) : Prop := 
 (cor_subset_ind xs ys /\ time_subset_ind xs ys) /\ (cor_proper_subset xs ys \/ time_proper_subset xs ys).
 
-Theorem spo_irr : forall (g1 : attackgraph measurement corruption) (x : list (g1.(state _ _) * g1.(state _ _)) ), ~ strict_partial_order x x.
+Theorem spo_irr : forall (g1 : attackgraph measurement adversary) (x : list (g1.(state _ _) * g1.(state _ _)) ), ~ strict_partial_order x x.
 Proof.
     intros. unfold strict_partial_order. unfold not. intros. intuition.
     + unfold cor_proper_subset in H0; invc H0; intuition.
     + unfold time_proper_subset in H0; invc H0; intuition.
 Qed.
 
-Theorem spo_asym : forall (g1 g2 : attackgraph measurement corruption)  (x : list (g1.(state _ _) * g1.(state _ _)) ) (y : list (g2.(state _ _) * g2.(state _ _)) ), strict_partial_order x y -> ~ strict_partial_order y x.
+Theorem spo_asym : forall (g1 g2 : attackgraph measurement adversary)  (x : list (g1.(state _ _) * g1.(state _ _)) ) (y : list (g2.(state _ _) * g2.(state _ _)) ), strict_partial_order x y -> ~ strict_partial_order y x.
 Proof.
     intros. unfold strict_partial_order in *. unfold not. intros. intuition.
     + unfold cor_proper_subset in H; invc H; intuition.
@@ -519,7 +519,7 @@ Qed.
 Ltac try_left := left; eapply cor_trans; eauto.
 Ltac try_right := right; eapply time_trans; eauto.
 
-Theorem spo_trans : forall (g1 g2 g3 : attackgraph measurement corruption) (xs : list (g1.(state _ _) * g1.(state _ _)) ) (ys : list (g2.(state _ _) * g2.(state _ _)) ), 
+Theorem spo_trans : forall (g1 g2 g3 : attackgraph measurement adversary) (xs : list (g1.(state _ _) * g1.(state _ _)) ) (ys : list (g2.(state _ _) * g2.(state _ _)) ), 
 strict_partial_order xs ys -> 
 forall (zs : list (g3.(state _ _) * g3.(state _ _)) ), strict_partial_order ys zs -> 
 strict_partial_order xs zs.
@@ -566,9 +566,9 @@ Module m3b.
     | ms : measurement
     | ms4 : measurement.
     
-    Inductive corruption : Type :=
-    | sys : corruption
-    | ker : corruption.
+    Inductive adversary : Type :=
+    | sys : adversary
+    | ker : adversary.
     
     Inductive state_m3b : Type :=
     | s : state_m3b 
@@ -576,7 +576,7 @@ Module m3b.
     | m : state_m3b
     | m4 : state_m3b.
     
-    Definition label_m3b (st : state_m3b) : measurement + corruption :=
+    Definition label_m3b (st : state_m3b) : measurement + adversary :=
     match st with
     | s => inr sys
     | k => inr ker
@@ -591,7 +591,7 @@ Module m3b.
         nil.
     
     
-    Definition m3b : attackgraph measurement corruption := 
+    Definition m3b : attackgraph measurement adversary := 
     {|
         state := state_m3b ;
         steps := steps_m3b ;
@@ -600,7 +600,7 @@ Module m3b.
     
     Lemma eqDec_measurement : forall (x y : measurement), {x = y} + {x <> y}.
     Proof. destruct x, y; try (left; reflexivity); try (right; intros contra; inversion contra). Qed.
-    Lemma eqDec_corruption : forall (x y : corruption), {x = y} + {x <> y}.
+    Lemma eqDec_adversary : forall (x y : adversary), {x = y} + {x <> y}.
     Proof. destruct x, y; try (left; reflexivity); try (right; intros contra; inversion contra). Qed.
     Lemma eqDec_state : forall (x y : m3b.(state _ _)), {x = y} + {x <> y}.
     Proof. destruct x, y; try (left; reflexivity); try (right; intros contra; inversion contra). Qed.
@@ -659,9 +659,9 @@ Inductive measurement : Type :=
 | ms : measurement
 | ms4 : measurement.
 
-Inductive corruption : Type :=
-| sys : corruption
-| ker : corruption.
+Inductive adversary : Type :=
+| sys : adversary
+| ker : adversary.
 
 Inductive state_m2c : Type :=
 | s : state_m2c
@@ -670,7 +670,7 @@ Inductive state_m2c : Type :=
 | m' : state_m2c
 | m4 : state_m2c.
 
-Definition label_m2c (st : state_m2c) : measurement + corruption :=
+Definition label_m2c (st : state_m2c) : measurement + adversary :=
 match st with
 | s => inr sys
 | k => inr ker
@@ -698,28 +698,28 @@ Definition steps_m2a : list (state_m2c * state_m2c) :=
     nil.
 
 
-Definition m2c : attackgraph measurement corruption := 
+Definition m2c : attackgraph measurement adversary := 
 {|
     state := state_m2c ;
     steps := steps_m2c ;
     label := label_m2c
 |}.
 
-Definition m2b : attackgraph measurement corruption := 
+Definition m2b : attackgraph measurement adversary := 
 {|
     state := state_m2c ;
     steps := steps_m2b ;
     label := label_m2c
 |}.
 
-Definition m2a : attackgraph measurement corruption := 
+Definition m2a : attackgraph measurement adversary := 
 {|
     state := state_m2c ;
     steps := steps_m2a ;
     label := label_m2c
 |}.
 
-Definition m2a_nil : attackgraph measurement corruption := 
+Definition m2a_nil : attackgraph measurement adversary := 
 {|
     state := state_m2c ;
     steps := nil ;
@@ -729,7 +729,7 @@ Definition m2a_nil : attackgraph measurement corruption :=
 
 Lemma eqDec_measurement : forall (x y : measurement), {x = y} + {x <> y}.
 Proof. destruct x, y; try (left; reflexivity); try (right; intros contra; inversion contra). Qed.
-Lemma eqDec_corruption : forall (x y : corruption), {x = y} + {x <> y}.
+Lemma eqDec_adversary : forall (x y : adversary), {x = y} + {x <> y}.
 Proof. destruct x, y; try (left; reflexivity); try (right; intros contra; inversion contra). Qed.
 Lemma eqDec_state : forall (x y : m2c.(state _ _)), {x = y} + {x <> y}.
 Proof. destruct x, y; try (left; reflexivity); try (right; intros contra; inversion contra). Qed.
@@ -798,10 +798,10 @@ Inductive measurement : Type :=
 | ms : measurement
 | ms4 : measurement.
 
-Inductive corruption : Type :=
-| sys : corruption
-| vc : corruption
-| cc : corruption.
+Inductive adversary : Type :=
+| sys : adversary
+| vc : adversary
+| cc : adversary.
 
 Inductive state_m5c : Type :=
 | s : state_m5c
@@ -811,7 +811,7 @@ Inductive state_m5c : Type :=
 | m' : state_m5c
 | m4 : state_m5c.
 
-Definition label_m5c (st : state_m5c) : measurement + corruption :=
+Definition label_m5c (st : state_m5c) : measurement + adversary :=
 match st with
 | s => inr sys
 | v => inr vc
@@ -829,7 +829,7 @@ Definition steps_m5c : list (state_m5c * state_m5c) :=
     (s, m4) ::
     nil.
 
-Definition m5c : attackgraph measurement corruption := 
+Definition m5c : attackgraph measurement adversary := 
 {|
     state := state_m5c ;
     steps := steps_m5c ;
@@ -845,7 +845,7 @@ Definition steps_m5c' : list (state_m5c * state_m5c) :=
     nil.
 
 (* new graph that would be proper subset *)
-Definition m5c' : attackgraph measurement corruption := 
+Definition m5c' : attackgraph measurement adversary := 
 {|
     state := state_m5c ;
     steps := steps_m5c' ;
@@ -854,7 +854,7 @@ Definition m5c' : attackgraph measurement corruption :=
 
 Lemma eqDec_measurement : forall (x y : measurement), {x = y} + {x <> y}.
 Proof. destruct x, y; try (left; reflexivity); try (right; intros contra; inversion contra). Qed.
-Lemma eqDec_corruption : forall (x y : corruption), {x = y} + {x <> y}.
+Lemma eqDec_adversary : forall (x y : adversary), {x = y} + {x <> y}.
 Proof. destruct x, y; try (left; reflexivity); try (right; intros contra; inversion contra). Qed.
 Lemma eqDec_state : forall (x y : m5c.(state _ _)), {x = y} + {x <> y}.
 Proof. destruct x, y; try (left; reflexivity); try (right; intros contra; inversion contra). Qed.
