src/coq_formalism/compare.v
@@ -19,7 +19,7 @@ Require Import Order.set_order.
 Section Compare.
 
   Context {measurement : Type}.
-  Context {corruption : Type}. 
+  Context {adversary : Type}. 
 
   (* 4 mutually exclusive ordering relations 
    * less than or equal to 
@@ -33,7 +33,7 @@ Section Compare.
   | eq
   | incomp. 
 
-  Inductive compare (g1 g2 : list (attackgraph measurement corruption)) : ord -> Prop :=
+  Inductive compare (g1 g2 : list (attackgraph measurement adversary)) : ord -> Prop :=
   | lte' : supports g1 g2 -> compare g1 g2 lte
   | gte' : supports g2 g1 -> compare g1 g2 gte
   | eq' : set_eq g1 g2 -> compare g1 g2 eq
