src/coq_formalism/set_equiv.v
@@ -19,9 +19,9 @@ Require Import Coq.Program.Equality.
 Section Set_Equiv. 
 
 Context {measurement : Type}.
-Context {corruption : Type}.
+Context {adversary : Type}.
 
-Definition set_eq (SS : list (attackgraph measurement corruption)) (TT : list (attackgraph measurement corruption)) :=  supports_iso SS TT /\ supports_iso TT SS.
+Definition set_eq (SS : list (attackgraph measurement adversary)) (TT : list (attackgraph measurement adversary)) :=  supports_iso SS TT /\ supports_iso TT SS.
 
 (* Prove properties of equivalence relation 
 * reflexivity 
